\subsection*{9.28}
$$\tau_1 (x) = \frac{1 + \cos \Omega x}{2}$$
$$\tau_2 (x) = e^{i m \cos \Omega x}$$
Вплотную:
$$E = E_0 \tau_1 \tau_2 = E_0 2 (\frac{1 + \cos \Omega x}{2} \cdot e^{i m \cos \Omega x}) = E_0  \frac{1 + \cos \Omega x}{2} (1 + m\cos \Omega x) =$$
$$= \frac{E_0}{2} + \frac{E_0}{2} i m \cos^2 \Omega x + \frac{E_0}{2}(\cos \Omega x + im \cos \Omega x) = $$
$$= \frac{E_0}{2} + E_0 im  \frac{\cos 2 \Omega x + 1}{2} + \frac{E_0}{4} (e^{i \Omega x} + e^{-i \Omega x} + m e^{-i \Omega x + \frac{\pi i}{2}} + me^{i \Omega x + \frac{\pi i}{2}}) $$
$E_{+1} = E_{-1}$ и $I_{-1} = I_{+1}$\\
$$E_0  \frac{1 + \cos (\Omega x - \frac{\pi}{2})}{2} (1 + im\cos \Omega x)$$
$$E_{-1} = \frac{E_0}{4} (e^{i \Omega x - \frac{\pi i }{2}} + im e^{i \Omega x}) = \frac{E_0}{4} (1 + m e^{-i (\Omega x - \frac{\pi}{2})})$$
$$\frac{E_1}{E_{-1}} = \frac{1-m}{1+m}; \  \frac{I_1}{I_{-1}} = \frac{(1-m)^2}{(1+m)^2} \approx 1 - 4m $$